wip: normal form progress

tests/playground/int_exhaust_test.lean
@@ -1,83 +1,234 @@
-/-
+import Lean.Util.TestNormalForms
 
-namespace IntTest
+open Lean
+open Lean.Elab.Command (CommandElab)
+open Lean.Test.NormalForms
+
+namespace Nat
+
+attribute [simp] mod_one
+
+end Nat
+
+namespace Int
+
+attribute [simp] emod_self
+
+@[simp] theorem zero_bdiv : bdiv 0 n = 0 := by sorry
+
+@[simp] theorem bdiv_one : bdiv m 1 = 0 := by sorry
+
+end Int
 
 inductive NumType where
 | nat
 | int
-deriving BEq, Hashable
+deriving BEq, Hashable, Inhabited, Repr
 
-inductive NumVal where
-| add (x y : NumVal) (tp : NumType)
-| var (d : VarDecl NumType)
-| natLit (n : Nat)
-deriving Inhabited
+protected def NumType.render [Monad M] [MonadQuotation M] (v : NumType) : M Term := do
+  match v with
+  | nat => `(Nat)
+  | int => `(Int)
 
-namespace NumVal
+inductive  DivMode where
+| divNat
+| edivInt
+| fdivInt
+| tdivInt
+| bdivInt
+deriving BEq, Repr
+
+def DivMode.typeOf (m : DivMode) : NumType :=
+  match m with
+  | divNat => .nat
+  | edivInt => .int
+  | fdivInt => .int
+  | tdivInt => .int
+  | bdivInt => .int
+
+inductive NumTerm where
+  | var (d : VarDecl NumType)
+  | lit (n : Nat) (tp : NumType)
+  | natToInt (x : NumTerm)
+  | intToNat (x : NumTerm)
+  | add (x y : NumTerm) (tp : NumType)
+  | sub (x y : NumTerm) (tp : NumType)
+  | neg (x : NumTerm) (tp : NumType)
+  | mul (x y : NumTerm) (tp : NumType)
+  | div (x y : NumTerm) (m : DivMode)
+  | mod (x y : NumTerm) (m : DivMode)
+  deriving BEq, Inhabited, Repr
+
+namespace NumTerm
 
 open NumType
 
-def addOp (tp : NumType) := mkOp [tp, tp] tp fun a => add (a[0]!) (a[1]!) tp
-
-def natLitOp (n : Nat) := mkOp [] nat fun _ => natLit n
-
-protected def typeOf (v : NumVal) : NumType :=
+partial def map (f : NumTerm → NumTerm) (v : NumTerm) : NumTerm :=
   match v with
-  | add _ _ tp => tp
-  | var d => d.type
-  | natLit _ => .nat
-
-instance : HasType NumVal NumType where
-  typeOf := NumVal.typeOf
-
-protected def render [Monad M] [MonadQuotation M] (v : NumVal) : M Term :=
-  match v with
-  | var d => do pure d.ident
-  | add x y _ => do `($(←x.render) + $(←y.render))
-  | natLit n => do `(($(Syntax.mkNumLit (toString n)) : Nat))
-
-instance : Value NumVal where
-  render := NumVal.render
-
-partial def map (f : NumVal → NumVal) (v : NumVal) : NumVal :=
-  match v with
+  | var _ | lit _ _ => v
+  | natToInt x => natToInt (f x)
+  | intToNat x => intToNat (f x)
   | add x y tp => add (f x) (f y) tp
-  | var d => var d
-  | natLit n => natLit n
+  | sub x y tp => sub (f x) (f y) tp
+  | neg x tp => neg (f x) tp
+  | mul x y tp => mul (f x) (f y) tp
+  | div x y op => div (f x) (f y) op
+  | mod x y op => mod (f x) (f y) op
 
-partial def simp (v : NumVal) : NumVal :=
+protected def typeOf (v : NumTerm) : NumType :=
+  match v with
+  | var d => d.type
+  | lit _ tp => tp
+  | natToInt _ => .int
+  | intToNat _ => .nat
+  | add _ _ tp => tp
+  | sub _ _ tp => tp
+  | neg _   tp => tp
+  | mul _ _ tp => tp
+  | div _ _ op => op.typeOf
+  | mod _ _ op => op.typeOf
+
+protected def render [Monad M] [MonadQuotation M] (v : NumTerm) : M Term := do
+  match v with
+  | var d => pure d.ident
+  | lit n tp => `(($(Syntax.mkNumLit (toString n)) : $(←tp.render)))
+  | natToInt x => `((($(←x.render) : Nat) : Int))
+  | intToNat x => `((($(←x.render) : Int) : Nat))
+  | add x y tp => `((($(←x.render) + $(←y.render)) : $(←tp.render)))
+  | sub x y _ => `($(←x.render) - $(←y.render))
+  | neg x _   => `(- $(←x.render))
+  | mul x y _ => `($(←x.render) * $(←y.render))
+  | div x y op =>
+    match op with
+    | .divNat  => `($(←x.render) / $(←y.render))
+    | .edivInt => `($(←x.render) / $(←y.render))
+    | .fdivInt => `(Int.fdiv $(←x.render) $(←y.render))
+    | .tdivInt => `(Int.div  $(←x.render) $(←y.render))
+    | .bdivInt => `(Int.bdiv $(←x.render) $(←y.render))
+  | mod x y op =>
+    match op with
+    | .divNat  => `($(←x.render) % $(←y.render))
+    | .edivInt => `($(←x.render) % $(←y.render))
+    | .fdivInt => `(Int.fmod $(←x.render) $(←y.render))
+    | .tdivInt => `(Int.mod  $(←x.render) $(←y.render))
+    | .bdivInt => `(Int.bmod $(←x.render) $(←y.render))
+
+instance : GenTerm NumTerm NumType where
+  render := NumTerm.render
+  mkVar := NumTerm.var
+
+def intLit (i : Int) : NumTerm :=
+  if i < 0 then
+    neg (lit ((- i).toNat) .int) .int
+  else
+    lit i.toNat .int
+
+partial def simp (v : NumTerm) : NumTerm :=
   let v := map simp v
   match v with
-  | add x y _ =>
+  | natToInt x =>
+    (match x with
+    | lit n _ => lit n .int
+    | add x y _ => add (natToInt x) (natToInt y) .int
+    | mul x y _ => mul (natToInt x) (natToInt y) .int
+    | div x y _ => div (natToInt x) (natToInt y) .edivInt
+    | mod x y _ => mod (natToInt x) (natToInt y) .edivInt
+    | var _ | sub _ _ _ | neg _ _ | intToNat _ | natToInt _ => v)
+  | add x y tp =>
     match x, y with
---    | x, natLit 0 => x
---    | natLit 0, y => y
+    | x, lit 0 _ => x
+    | lit 0 _, y => y
+    | lit i _, lit j _ => lit (i+j) tp
     | _, _ => v
+  | sub x y tp =>
+    match x, y, tp with
+    | x, lit 0 _, _ => x
+    | lit i _, lit j _, .nat => lit (i-j) tp
+    | lit i _, lit j _, .int => intLit ((i : Int) - (j : Int))
+    | lit 0 _, _, .nat => lit 0 .nat
+    | lit 0 _, y, .int => simp (neg y .int)
+    | x, y, _ =>
+      if x == y then
+        .lit 0 tp
+      else
+        v
+  | neg x _ =>
+    match x with
+    | lit n _ => intLit (- (Int.ofNat n))
+    | _ => v
+  | mul x y tp =>
+    match x, y with
+    | _, lit 0 _ => y
+    | lit 0 _, _ => x
+    | _, lit 1 _ => x
+    | lit 1 _, _ => y
+    | lit i _, lit j _ => lit (i*j) tp
+    | _, _ => v
+  | div x y _op =>
+    if let lit 0 _ := x then
+      x
+    else if let lit 0 _ := y then
+      y
+    else if let lit 1 _ := y then
+      x
+    else
+      v
+  | mod x y op =>
+    if let lit 0 _ := x then
+      x
+    else if let lit 0 _ := y then
+      x
+    else if let lit 1 _ := y then
+      lit 0 op.typeOf
+    else if x == y then
+      lit 0 op.typeOf
+    else
+      v
   | _ => v
 
-end NumVal
+partial def simpv (u : NumTerm) : NumTerm :=
+  let v := simp u
+  if v.typeOf == u.typeOf then
+    v
+  else
+    panic! s!"{repr u} has changed types."
 
-open NumVal
+def litOp (n : Nat) (tp : NumType) := mkOp [] tp fun _ => lit n tp
+def addOp (tp : NumType) := mkOp [tp, tp] tp fun a => add (a[0]!) (a[1]!) tp
+def subOp (tp : NumType) := mkOp [tp, tp] tp fun a => sub (a[0]!) (a[1]!) tp
+def negOp (tp : NumType) := mkOp [tp] tp fun a => neg (a[0]!) tp
+def mulOp (tp : NumType) := mkOp [tp, tp] tp fun a => mul (a[0]!) (a[1]!) tp
+def divOp (op : DivMode) (dtp := op.typeOf) := let tp := op.typeOf; mkOp [tp, dtp] tp fun a => div (a[0]!) (a[1]!) op
+def modOp (op : DivMode) (dtp := op.typeOf) := let tp := op.typeOf; mkOp [tp, dtp] tp fun a => mod (a[0]!) (a[1]!) op
+
+end NumTerm
+
+open NumTerm
 
 syntax:lead (name := intTestElab) "#intTest" : command
 
 @[command_elab intTestElab]
-def elabIntTest : CommandElab := fun stx => do
-  let stats : GenStats := { maxTermSize := 7, maxDepth := 2, maxVarCount := 3 }
-  let types := #[.nat, .int]
+def elabIntTest : CommandElab := fun _stx => do
+  let types : List NumType := [.nat, .int]
   let ops := [
-      addOp .nat,
-      natLitOp 0
+      litOp 0 .nat,
+      litOp 1 .nat,
+      litOp 0 .int,
+      litOp 1 .int,
+      addOp .nat, addOp .int,
+      subOp .nat, subOp .int,
+      negOp .int,
+      mulOp .nat, mulOp .int,
+      divOp .divNat, divOp .edivInt, divOp .fdivInt, divOp .tdivInt, divOp .bdivInt .nat,
+      modOp .divNat, modOp .edivInt, modOp .fdivInt, modOp .tdivInt, divOp .bdivInt .nat,
   ]
-  let varGen : List (NumType × CoreM Command) := [
+  let vars : List (NumType × CoreM Command) := [
       (.nat, `(variable (n : Nat))),
       (.int, `(variable (i : Int)))
   ]
-  let tac : Syntax.Tactic ← `(tactic|try simp)
-  runGen stx NumVal.simp varGen NumVal.var stats types ops tac
+  let stats : GenStats := { maxTermSize := 7, maxDepth := 2, maxVarCount := 3 }
+  testNormalForms types ops vars NumTerm.simpv stats
 
---set_option pp.all true
---#intTest
-
-end IntTest
--/
+--set_option pp.coercions false
+--set_option pp.explicit true
+#intTest
