exprGen.lean
@@ -1,0 +1,187 @@
+import Lean
+
+section
+open Lean Elab Meta Command
+
+syntax:lead (name := metaliftElab) "#metalift" ident : command
+
+
+def nameToIdent (nm : Name) : TermElabM Syntax.Term :=
+  match nm with
+  | .anonymous => `(Name.anonymous)
+  | .str nm r => do `(Name.str $(←nameToIdent nm) $(Syntax.mkStrLit r))
+  | .num nm r => do `(Name.num $(←nameToIdent nm) $(Syntax.mkNumLit (toString r)))
+
+@[command_elab metaliftElab]
+def elabGenTest : CommandElab := fun stx => do
+  let `(command|#metalift $d) := stx | throwUnsupportedSyntax
+  let typeName := d.getId
+  let indVal ← getConstInfoInduct typeName
+  let recName := typeName.str "rec"
+  let _ ← getConstInfoRec recName
+  let toExprIdent := mkIdent (typeName.str "toExpr")
+  let args ←
+    liftTermElabM do
+      let mut args : TSyntaxArray `term := #[]
+      for c in indVal.ctors do
+        let ctp ← inferType (.const c [])
+        let meta ← forallMetaTelescope ctp
+        let ctorArgVars := meta.1
+
+        let n := ctorArgVars.size
+        log m!"Constructor {c} {n}"
+        let mut val ← `(term|Lean.Expr.const $(←nameToIdent c) [])
+        --let mut val ← `(term|sorry)
+        let mut ctorArgs : Array Ident := .mkEmpty n
+        for i in [0:n] do
+          let argVar := ctorArgVars[i]!
+          let argType ← inferType argVar
+          let nmIdent := mkIdent s!"b{i}"
+          ctorArgs := ctorArgs.push nmIdent
+          let .const argTypeName [] := argType | throwError "Expected constant {argType}"
+          let argVal ←
+                if argTypeName == typeName then
+                  `($toExprIdent $nmIdent)
+                else if argTypeName == ``Nat then
+                  `(Lean.ToExpr.toExpr $nmIdent)
+                else
+                  throwError "Unexpected constant {argType}"
+          val := ←`(term|Lean.Expr.app $val $argVal)
+        for i in [0:n] do
+          let nmIdent := ctorArgs[n-1-i]!
+          val := ←`(term| fun $nmIdent => $val)
+        ctorArgs := ctorArgs.reverse
+
+        args := args.push val
+      pure args
+  let typeIdent := mkIdent typeName
+  let casesOnIdent := mkIdent (typeName.str "casesOn")
+  elabCommand (←`(command|
+    def $toExprIdent (t : $typeIdent) := @$casesOnIdent (fun _ => Lean.Expr) t $args*))
+
+end
+
+inductive Term where
+| cns (x : Nat)
+| add (x y : Term)
+
+
+#print
+#metalift Bool
+#metalift Term
+
+#print Term.toExpr
+--set_option pp.all true
+#eval Term.toExpr (.cns 0)
+#print BoolVal.bar.match_1
+
+partial def listOfExprAux (a : List Expr) (e : Expr) : MetaM (List Expr) := do
+  let e ← whnf e
+  match e with
+  | .app (.app (.app (.const ``List.cons [_u]) _tp) h) e =>
+    listOfExprAux (h :: a) e
+  | .app (.const ``List.nil [_u]) _tp =>
+    pure a.reverse
+  | _ =>
+    throwError s!"Could not parse {e}"
+
+def listOfExpr (e : Expr) : MetaM (List Expr) := listOfExprAux [] e
+
+structure Match where
+  eq : Expr
+
+instance : BEq Match where
+  beq _ _ := false -- FIXME?
+
+def matchDtConfig : WhnfCoreConfig := {}
+
+def addMatchProp (d : DiscrTree Match) (p : Expr) : MetaM (DiscrTree Match) := do
+  let pa ← withReducible (forallMetaTelescopeReducing p)
+  let eq := pa.2.2
+  let pat ←
+    match eq with
+    | .app (.app (.app (.const `Eq [_]) _) lhs) _ => pure lhs
+    | _ =>
+      throwError m!"Could not interpret {eq} as equation."
+  let keys ←  DiscrTree.mkPath pat matchDtConfig
+  let ma : Match := { eq }
+  pure <| d.insertCore keys ma
+
+def mkDiscrTree (rules : List Expr) : MetaM (DiscrTree Match):= do
+  rules.foldlM (init := DiscrTree.empty) addMatchProp
+
+/-run_meta do
+  let l ← listOfExpr (.const ``Rules [])
+  let t ← mkDiscrTree l
+  throwError s!"Parsed {l.length}"
+  pure ()
+
+partial def simp_from_rules [h : ToExpr BoolVal] (rules : List Prop) (v : BoolVal) : MetaM BoolVal := do
+  let t ← mkDiscrTree rules
+  let e := toExpr v
+
+
+  -- Discrimination tree
+  -- Lift
+  sorry
+
+-/
+
+namespace Quot
+
+structure Context where
+  mainModule : Name
+  ref : Syntax
+  currMacroScope : MacroScope
+
+
+end Quot
+
+def QuotM := ReaderT Quot.Context (StateM MacroScope)
+
+namespace QuotM
+
+instance : Monad QuotM := inferInstanceAs (Monad (ReaderT _ _))
+local instance : MonadReader Quot.Context QuotM := inferInstanceAs (MonadReader _ (ReaderT _ _))
+local instance : MonadState MacroScope QuotM := inferInstanceAs (MonadState _ (ReaderT _ _))
+
+protected def withFreshMacroScope (m : QuotM α) : QuotM α := do
+  let fresh ← modifyGet (fun s => (s, s + 1))
+  ReaderT.adapt ({· with currMacroScope := fresh }) m
+
+instance : MonadQuotation QuotM where
+  getRef := return (← read).ref
+  withRef ref := ReaderT.adapt ({ · with ref })
+  getCurrMacroScope := return (← read).currMacroScope
+  getMainModule := return (← read).mainModule
+  withFreshMacroScope := QuotM.withFreshMacroScope
+
+end QuotM
+
+inductive App (α : Type) where
+| mkApp (op : QuotM Term) (args : Array α)
+
+export App (mkApp)
+
+/-
+def getConstInfoRec [Monad m] [MonadEnv m] [MonadError m] (constName : Name) : m RecursorVal := do
+  match (← getConstInfo constName) with
+  | ConstantInfo.recInfo v => pure v
+  | _                      => throwError "'{mkConst constName}' is not a recursor"
+-/
+
+def Rules : List Prop := [
+  ∀tp,     decide (trueVal tp)  = trueVal bool,
+  ∀tp,     decide (falseVal tp) = falseVal bool,
+  ∀tp x,   decide (not x tp) = decide x,
+  ∀tp x y, decide (and x y tp) = (decide x &&& decide y),
+  ∀tp x y, decide (or  x y tp) = (decide x ||| decide y),
+  ∀x y,    decide (implies x y) = ~(decide x) ||| decide y,
+  ∀x y,    decide (eq x y .iffProp) = eq (decide x) (decide y) .beqBool,
+  ∀x op,   decide (eq x (trueVal  bool) op) = x,
+  ∀x op,   decide (eq x (falseVal bool) op) = ~x,
+  ∀x y,    decide (eq x y .eqBool)  = eq x y .beqBool,
+  ∀x y,    decide (eq x y .eqProp)  = eq (decide x) (decide y) .beqBool,
+  ∀x y,    decide (eq x y .iffProp) = eq (decide x) (decide y) .beqBool,
+  ∀c t f,  decide (ite c t f .iteProp) = ite c (decide t) (decide f) .iteBool
+  ]
